---
{"dg-publish":true,"permalink":"/leeds-university/computer-science/compulsory-modules/discrete-mathematics/1-combinatorics/1-combinatorics/"}
---


<div class="transclusion internal-embed is-loaded"><a class="markdown-embed-link" href="/leeds-university/computer-science/compulsory-modules/discrete-mathematics/1-combinatorics/1-1-basic-counting-principles/1-1-basic-counting-principles/" aria-label="Open link"><svg xmlns="http://www.w3.org/2000/svg" width="24" height="24" viewBox="0 0 24 24" fill="none" stroke="currentColor" stroke-width="2" stroke-linecap="round" stroke-linejoin="round" class="svg-icon lucide-link"><path d="M10 13a5 5 0 0 0 7.54.54l3-3a5 5 0 0 0-7.07-7.07l-1.72 1.71"></path><path d="M14 11a5 5 0 0 0-7.54-.54l-3 3a5 5 0 0 0 7.07 7.07l1.71-1.71"></path></svg></a><div class="markdown-embed">





<div class="transclusion internal-embed is-loaded"><a class="markdown-embed-link" href="/leeds-university/computer-science/compulsory-modules/discrete-mathematics/1-combinatorics/1-1-basic-counting-principles/the-multiplication-principle/#the-multiplication-principle-for-counting-procedures" aria-label="Open link"><svg xmlns="http://www.w3.org/2000/svg" width="24" height="24" viewBox="0 0 24 24" fill="none" stroke="currentColor" stroke-width="2" stroke-linecap="round" stroke-linejoin="round" class="svg-icon lucide-link"><path d="M10 13a5 5 0 0 0 7.54.54l3-3a5 5 0 0 0-7.07-7.07l-1.72 1.71"></path><path d="M14 11a5 5 0 0 0-7.54-.54l-3 3a5 5 0 0 0 7.07 7.07l1.71-1.71"></path></svg></a><div class="markdown-embed">



###### The Multiplication Principle for Counting Procedures
If a sequence can be described as a sequence of ${\color{red} n}$ *independent* steps, with ${\color{blue} i}_{1}$ possible outcomes for the first step, ${\color{blue} i}_{2}$ possible outcomes for the second step, $\dots$, and ${\color{blue} i}_{{\color{red} n}}$ possible outcomes for the ${\color{red} n}^{th}$ step, then the total number of composite outcomes of the procedure is ${\color{blue} i}_{1}{\color{blue} i}_{2}\dots{\color{blue} i}_{{\color{red} n}}$

</div></div>


<div class="transclusion internal-embed is-loaded"><a class="markdown-embed-link" href="/leeds-university/computer-science/compulsory-modules/discrete-mathematics/1-combinatorics/1-1-basic-counting-principles/the-addition-principle/#the-addition-principle-for-counting-procedures" aria-label="Open link"><svg xmlns="http://www.w3.org/2000/svg" width="24" height="24" viewBox="0 0 24 24" fill="none" stroke="currentColor" stroke-width="2" stroke-linecap="round" stroke-linejoin="round" class="svg-icon lucide-link"><path d="M10 13a5 5 0 0 0 7.54.54l3-3a5 5 0 0 0-7.07-7.07l-1.72 1.71"></path><path d="M14 11a5 5 0 0 0-7.54-.54l-3 3a5 5 0 0 0 7.07 7.07l1.71-1.71"></path></svg></a><div class="markdown-embed">



###### The Addition Principle for Counting Procedures
If a procedure can be broken up into ${\color{red} m}$ events or cases whose [[Leeds University/Computer Science/Compulsory Modules/Fundamental Math Concepts/5. Set Theory/5.1 Sets\|sets]] of outcomes are mutually exclusive, with ${\color{blue} j}_{1}$ possible outcomes for the first event, ${\color{blue} j}_{2}$ possible outcomes for the second event, $\dots$, and ${\color{blue} j}_{\color{red} m}$ for the ${\color{red} m}^{th}$ event, then the total number of outcomes of the procedure is ${\color{blue} j}_{1}+{\color{blue} j}_{2}+\dots+{\color{blue} j}_{{\color{red} m}}$

</div></div>



</div></div>


<div class="transclusion internal-embed is-loaded"><a class="markdown-embed-link" href="/leeds-university/computer-science/compulsory-modules/discrete-mathematics/1-combinatorics/1-2-selections/1-2-selections/" aria-label="Open link"><svg xmlns="http://www.w3.org/2000/svg" width="24" height="24" viewBox="0 0 24 24" fill="none" stroke="currentColor" stroke-width="2" stroke-linecap="round" stroke-linejoin="round" class="svg-icon lucide-link"><path d="M10 13a5 5 0 0 0 7.54.54l3-3a5 5 0 0 0-7.07-7.07l-1.72 1.71"></path><path d="M14 11a5 5 0 0 0-7.54-.54l-3 3a5 5 0 0 0 7.07 7.07l1.71-1.71"></path></svg></a><div class="markdown-embed">




Suppose that a child is offered a bag containing three types of sweets, aniseed drops $({\color{red} A})$, butter mints $({\color{lightgreen} B})$ and cherry drops $({\color{blue} C})$. In how many ways can the child ***select*** two sweets?

This problem is not defined well, since we are not told:
- whether or not the same type of sweet can be selected twice, i.e. is ${\color{red} AA}$ allowed?
- whether the order matter, i.e. is ${\color{red} A}{\color{lightgreen} B}$ to be treated the same as ${\color{lightgreen} B}{\color{red} A}$, or not?

There are 4 cases to consider:
1. **Repeats are allowed** and **order matters**. This gives 9 possibilities:
	- ${\color{red} A}{\color{red} A}, {\color{red} A}{\color{lightgreen} B}, {\color{red} A}{\color{blue} C}, {\color{lightgreen} B}{\color{red} A}, {\color{lightgreen} B}{\color{lightgreen} B}, {\color{lightgreen} B}{\color{blue} C}, {\color{blue} C}{\color{red} A}, {\color{blue} C}{\color{lightgreen} B}, {\color{blue} C}{\color{blue} C}$
	- [[Leeds University/Computer Science/Compulsory Modules/Discrete Mathematics/1. Combinatorics/1.2 Selections/1.2.3 Permutations with Unlimited Repetition\|Permutations with Unlimited Repetition]]
1. **Repeats are allowed** and **order *doesn’t* matter**. This gives 6 possibilities:
	- ${\color{red} A}{\color{red} A}, {\color{red} A}{\color{lightgreen} B}, {\color{red} A}{\color{blue} C}, {\color{lightgreen} B}{\color{lightgreen} B}, {\color{lightgreen} B}{\color{blue} C}, {\color{blue} C}{\color{blue} C}$
	- [[Leeds University/Computer Science/Compulsory Modules/Discrete Mathematics/1. Combinatorics/1.2 Selections/1.2.4 Combinations with Unlimited Repetition\|Combinations with Unlimited Repetition]]
1. **Repeats are *not* allowed** and **order matters**. This gives 6 possibilities
	- ${\color{red} A}{\color{lightgreen} B}, {\color{red} A}{\color{blue} C}, {\color{lightgreen} B}{\color{red} A}, {\color{lightgreen} B}{\color{blue} C}, {\color{blue} C}{\color{red} A}, {\color{blue} C}{\color{lightgreen} B}$
	- [[Leeds University/Computer Science/Compulsory Modules/Discrete Mathematics/1. Combinatorics/1.2 Selections/1.2.1 Permutations\|Permutations]]
2. **Repeats *are* not allowed** and **order *doesn’t* matter**. This give 3 possibilities
	- ${\color{red} A}{\color{lightgreen} B}, {\color{red} A}{\color{blue} C}, {\color{lightgreen} B}{\color{blue} C}$
	- [[Leeds University/Computer Science/Compulsory Modules/Discrete Mathematics/1. Combinatorics/1.2 Selections/1.2.2 Combinations\|Combinations]]


</div></div>


<div class="transclusion internal-embed is-loaded"><a class="markdown-embed-link" href="/leeds-university/computer-science/compulsory-modules/discrete-mathematics/1-combinatorics/1-3-binomial-coefficients-and-combinatorial-identities/1-3-binomial-coefficients-and-combinatorial-identities/" aria-label="Open link"><svg xmlns="http://www.w3.org/2000/svg" width="24" height="24" viewBox="0 0 24 24" fill="none" stroke="currentColor" stroke-width="2" stroke-linecap="round" stroke-linejoin="round" class="svg-icon lucide-link"><path d="M10 13a5 5 0 0 0 7.54.54l3-3a5 5 0 0 0-7.07-7.07l-1.72 1.71"></path><path d="M14 11a5 5 0 0 0-7.54-.54l-3 3a5 5 0 0 0 7.07 7.07l1.71-1.71"></path></svg></a><div class="markdown-embed">




At first glance the expression $({\color{lavender} a}+{\color{orange} b})^{\color{red} n}$ does not have much to do with [[Leeds University/Computer Science/Compulsory Modules/Discrete Mathematics/1. Combinatorics/1.2 Selections/1.2.2 Combinations\|Combinations]], but it turns out that we can obtain the [[Leeds University/Computer Science/Compulsory Modules/Fundamental Math Concepts/Fundamentals of Logic/Definitions/Formula\|formula]] for the expansion of $({\color{lavender} a}+{\color{orange} b})^{\color{red} n}$ by using the [[Leeds University/Computer Science/Compulsory Modules/Fundamental Math Concepts/Fundamentals of Logic/Definitions/Formula\|formula]] for ${\color{blue} k}$-[[Leeds University/Computer Science/Compulsory Modules/Discrete Mathematics/1. Combinatorics/1.2 Selections/1.2.2 Combinations\|combinations]] of ${\color{red} n}$ objects

$
\begin{align}
&({\color{lavender} a}+{\color{orange} b})^{3} \\
&=({\color{lavender} a}+{\color{orange} b})({\color{lavender} a}+{\color{orange} b})({\color{lavender} a}+{\color{orange} b}) \\
&={\color{lavender} a}{\color{lavender} a}{\color{lavender} a}+{\color{lavender} a}{\color{lavender} a}{\color{orange} b}+{\color{lavender} a}{\color{orange} b}{\color{lavender} a}+{\color{lavender} a}{\color{orange} b}{\color{orange} b}+{\color{orange} b}{\color{lavender} a}{\color{lavender} a}+{\color{orange} b}{\color{lavender} a}{\color{orange} b}+{\color{orange} b}{\color{orange} b}{\color{lavender} a}+{\color{orange} b}{\color{orange} b}{\color{orange} b} \\
&={\color{lavender} a}^{3}+3{\color{lavender} a}^{2}{\color{orange} b}+3{\color{lavender} a}{\color{orange} b}^{2}+{\color{orange} b}^{3}
\end{align}
$
**[[Leeds University/Computer Science/Compulsory Modules/Discrete Mathematics/1. Combinatorics/Theorems/Theorem 1.5\|Theorem 1.5]]**

<div class="transclusion internal-embed is-loaded"><a class="markdown-embed-link" href="/leeds-university/computer-science/compulsory-modules/discrete-mathematics/1-combinatorics/theorems/theorem-1-5/#definition" aria-label="Open link"><svg xmlns="http://www.w3.org/2000/svg" width="24" height="24" viewBox="0 0 24 24" fill="none" stroke="currentColor" stroke-width="2" stroke-linecap="round" stroke-linejoin="round" class="svg-icon lucide-link"><path d="M10 13a5 5 0 0 0 7.54.54l3-3a5 5 0 0 0-7.07-7.07l-1.72 1.71"></path><path d="M14 11a5 5 0 0 0-7.54-.54l-3 3a5 5 0 0 0 7.07 7.07l1.71-1.71"></path></svg></a><div class="markdown-embed">




If ${\color{lavender} a}$ and ${\color{orange} b}$ are real numbers and ${\color{red} n}$ is a positive integer, then $({\color{lavender} a}+{\color{orange} b})^{\color{red} n}=\sum\limits^{\color{red} n}_{{\color{blue} k}=0}\binom{{\color{red} n}}{{\color{blue} k}}{\color{lavender} a}^{{\color{red} n}-{\color{blue} k}}{\color{orange} b}^{\color{blue} k}$ 
###### *Proof*: $\color{white} ({\color{lavender} a}+{\color{orange} b})^{\color{red} n}=({\color{lavender} a}+{\color{orange} b})\dots({\color{lavender} a}+{\color{orange} b})\ ({\color{red} n}\text{ factors})$
In the expansion of $({\color{lavender} a}+{\color{orange} b})^{\color{red} n}$, a term of the form ${\color{lavender} a}^{{\color{red} n}-{\color{blue} k}}{\color{orange} b}^{\color{blue} k}$ arises from choosing ${\color{orange} b}$ from ${\color{blue} k}$ factors and ${\color{lavender} a}$ from the other ${\color{red} n}-{\color{blue} k}$ factors. This can be done in $\binom{{\color{red} n}}{{\color{blue} k}}$ ways. Thus ${\color{lavender} a}^{{\color{red} n}-{\color{blue} k}}{\color{orange} b}^{\color{blue} k}$ appears $\binom{{\color{red} n}}{{\color{blue} k}}$ times in the expansion. It follows that:
$
\begin{align}
&({\color{lavender} a}+{\color{orange} b})^{\color{red} n} \\
&={\tiny\binom{{\color{red} n}}{0}}{\color{lavender} a}^{{\color{red} n}-1}{\color{orange} b}^{1}+{\tiny\binom{{\color{red} n}}{2}}{\color{lavender} a}^{{\color{red} n}-2}{\color{orange} b}^{2}+\dots+{\tiny\binom{{\color{red} n}}{{\color{red} n}-1}}{\color{lavender} a}^{1}{\color{orange} b}^{{\color{red} n}-1}+{\tiny\binom{{\color{red} n}}{{\color{red} n}}}{\color{lavender} a}^{0}{\color{orange} b}^{\color{red} n} \\
&=\small\sum\limits^{\color{red} n}_{{\color{blue} k}=0}{\tiny\binom{{\color{red} n}}{{\color{blue} k}}}{\color{lavender} a}^{{\color{red} n}-{\color{blue} k}}{\color{orange} b}^{\color{blue} k}
\end{align}
$
The numbers $\binom{{\color{red} n}}{{\color{blue} k}}$ are known as *binomial coefficients* because they appear in the expansion of $({\color{lavender} a}+{\color{orange} b})^{\color{red} n}$


</div></div>


>[!example] 
>What is the coefficient of ${\color{lavender} x}^{12}{\color{orange} y}^{13}$ in the expansion of $({\color{lavender} x}+{\color{orange} y})^{25}$

$\binom{25}{13}=\frac{25!}{13!12!}$

>[!example]
>Find the coefficient of ${\color{lavender} x}^{4}{\color{orange} y} ^{5}$ in the expansion of $(2{\color{lavender} x}-{\color{orange} y})^{9}$

$(-1)^{5}\times\binom{9}{5}\times2^{4}=-2016$

>[!example] 
>Find the coefficient of ${\color{lavender} x}^{2}{\color{orange} y}^{3}{\color{lightgreen} z}^{4}$ in the expansion of $({\color{lavender} x}+{\color{orange} y}+{\color{lightgreen} z})^{9}$

Model as $({\color{lavender} x}+({\color{orange} y}+{\color{lightgreen} z}))^{9}$
$\binom{9}{7}({\color{orange} y}+{\color{lightgreen} z})^{7}$
$=\binom{9}{7}\binom{7}{4}=1260$

>[!example] 
>Prove that for a positive integer ${\color{red} n}$, $\sum\limits^{\color{red} n}_{{\color{blue} k}=0}\binom{{\color{red} n}}{{\color{blue} k}}=2^{\color{red} n}$

*Proof using the [[Leeds University/Computer Science/Compulsory Modules/Discrete Mathematics/1. Combinatorics/Theorems/Theorem 1.5\|Binomial Theorem]]*
$2^{\color{red} n}=(1+1)^{\color{red} n}=\sum\limits^{\color{red} n}_{{\color{blue} k}=0}\binom{{\color{red} n}}{{\color{blue} k}}1^{{\color{red} n}-{\color{blue} k}}1^{\color{blue} k}=\sum\limits^{\color{red} n}_{{\color{blue} k}=0}\binom{n}{k}$

*[[Leeds University/Computer Science/Compulsory Modules/Discrete Mathematics/1. Combinatorics/Definitions/Combinatorial Proof\|Combinatorial Proof]]*
A [[Leeds University/Computer Science/Compulsory Modules/Fundamental Math Concepts/5. Set Theory/5.1 Sets\|set]] with ${\color{red} n}$ elements has $2^{\color{red} n}$ different [[Leeds University/Computer Science/Compulsory Modules/Fundamental Math Concepts/5. Set Theory/Definitions/Definition 5.5 (Subsets and Supersets)\|subsets]]
Each subset has ${\color{blue} k}$ elements for ${\color{blue} k}\in\set{0,1,\dots,{\color{red} n}}$
There are $\binom{{\color{red} n}}{{\color{blue} k}}$ [[Leeds University/Computer Science/Compulsory Modules/Fundamental Math Concepts/5. Set Theory/Definitions/Definition 5.5 (Subsets and Supersets)\|subsets]] with ${\color{blue} k}$ elements
Therefore the total number of [[Leeds University/Computer Science/Compulsory Modules/Fundamental Math Concepts/5. Set Theory/Definitions/Definition 5.5 (Subsets and Supersets)\|subsets]] is $\sum\limits^{\color{red} n}_{{\color{blue} k}=0}\binom{{\color{red} n}}{{\color{blue} k}}$,
and hence $\sum\limits^{\color{red} n}_{{\color{blue} k}=0}\binom{{\color{red} n}}{{\color{blue} k}}=2^{\color{red} n}$


</div></div>


<div class="transclusion internal-embed is-loaded"><a class="markdown-embed-link" href="/leeds-university/computer-science/compulsory-modules/discrete-mathematics/1-combinatorics/1-4-the-pigeonhole-principle/1-4-the-pigeonhole-principle/" aria-label="Open link"><svg xmlns="http://www.w3.org/2000/svg" width="24" height="24" viewBox="0 0 24 24" fill="none" stroke="currentColor" stroke-width="2" stroke-linecap="round" stroke-linejoin="round" class="svg-icon lucide-link"><path d="M10 13a5 5 0 0 0 7.54.54l3-3a5 5 0 0 0-7.07-7.07l-1.72 1.71"></path><path d="M14 11a5 5 0 0 0-7.54-.54l-3 3a5 5 0 0 0 7.07 7.07l1.71-1.71"></path></svg></a><div class="markdown-embed">




The ***Pigeonhole Principle***  (or the *Dirichlet Principle*) is sometimes useful in answering the question:
<u>Is there an item having a given property?</u>

**Pigeonhole Principle**: If ${\color{red} n}$ pigeons fly into ${\color{blue} k}$ pigeonholes and ${\color{blue} k}\le {\color{red} n}$, then some pigeonhole contains *at least* two pigeons

**Example**:
>[!example] 
>Ten people have the first name Alice, Bernard and Charles, and last names Lee, Mc-Duff and Ng. Show that at least two people have the same first and last names.

There are $3\times3=9$ possible names for the 10 people. If we think of people as *pigeons* and the names as *pigeonholes*, we can consider the assignments of names to people as assigning pigeonholes to pigeons. By the **Pigeonhole Principle**, some name (pigeonhole) is assigned to at least two people (pigeons)

**Generalised Pigeonhole Principle**: If ${\color{red} n}$ pigeons fly into ${\color{blue} k}$ pigeonholes, then some pigeonhole contains *at least* $\empheqlceil\frac{{\color{red} n}}{{\color{blue} k}}\empheqrceil$ pigeons 
###### *Proof*:
Suppose that none of the pigeonholes contain more than $\empheqlceil\frac{{\color{red} n}}{{\color{blue} k}}\empheqrceil - 1$ pigeons. Then the total number of pigeons is at most ${\color{blue} k}(\empheqlceil\frac{{\color{red} n}}{{\color{blue} k}}\empheqrceil - 1)$, which is **always** less than ${\color{red} n}$

# <hr>

>[!example] 
>What is the minimum number of students required in a discrete maths class to be sure that at least 6 will receive the same grade, if there are 5 possible grades, A,B,C,D and F

$\empheqlceil\frac{{\color{red} n}}{{\color{blue} 5}}\empheqrceil=6$
${\color{red} n}=5(6-1)+1=25+1=26$




</div></div>

